src/lang/Local.v
@@ -170,6 +170,7 @@ Module Local.
       (TVIEW_WF: TView.wf lc.(tview))
       (TVIEW_CLOSED: TView.closed lc.(tview) mem)
       (PROMISES: Memory.le lc.(promises) mem)
+      (BOT: Memory.bot_none lc.(promises))
   .
   Hint Constructors wf.
 
