src/opt/SplitAcqRel.v
@@ -62,6 +62,7 @@ Proof.
   i. des.
   exploit Memory.promise_future; try apply PROMISE_SRC; eauto.
   { apply WF1_SRC. }
+  { apply WF1_SRC. }
   { destruct msg; ss. inv CLOSED. econs.
     eapply sim_memory_closed_opt_view; eauto. }
   i. des.
